Makefile
@@ -727,7 +727,6 @@ INSTALL_FILES=$(sort $(INSTALL_FILES_SRC) $(INSTALL_FILES_VO))
 
 # util/calc_install_files_refinedcc takes the directory name as the only argument
 RC_INSTALL_FILES_SRC=$(shell COMPCERT=$(COMPCERT) COMPCERT_INST_DIR=$(COMPCERT_INST_DIR) ZLIST=$(ZLIST) BITSIZE=$(BITSIZE) ARCH=$(ARCH) IGNORECOQVERSION=$(IGNORECOQVERSION) IGNORECOMPCERTVERSION=$(IGNORECOMPCERTVERSION) MAKE=$(MAKE) util/calc_install_files_refinedcc veric/make_compspecs.v refinedVST)
-RC_INSTALL_FILES_SRC+=veric/make_compspecs.v
 RC_INSTALL_FILES_VO=$(patsubst %.v,%.vo,$(RC_INSTALL_FILES_SRC))
 RC_INSTALL_FILES=$(sort $(RC_INSTALL_FILES_SRC) $(RC_INSTALL_FILES_VO))
 
